FGL: Revamp stack.lisp to support late bindings -- major stack with minor substacks

books/centaur/fgl/stack.lisp
@@ -38,35 +38,128 @@
 (local (include-book "std/lists/nth" :dir :system))
 (local (include-book "std/lists/resize-list" :dir :system))
 
+(local (include-book "std/util/termhints" :dir :system))
+(local (include-book "std/basic/arith-equivs" :dir :system))
+(local (include-book "arithmetic/top-with-meta" :dir :system))
+(local (include-book "std/stobjs/updater-independence" :dir :system))
+
+(local (in-theory (enable* acl2::arith-equiv-forwarding)))
+
 (local (fty::deflist gl-objectlist :elt-type gl-object :true-listp t))
 
-(local (in-theory (disable nth acl2::nth-when-zp update-nth)))
+(local (in-theory (disable nth acl2::nth-when-zp update-nth (tau-system))))
 
-;; A stack is (logically) just a list of stack-frames, where each frame has a
-;; binding list BINDINGS, an objectlist SCRATCH, and a debug field (type yet
-;; undetermined).  The topmost stack frame is the first one.
+(local (std::add-default-post-define-hook :fix))
+
+;; This book defines a stack containing "major frames", each containing a stack
+;; of "minor frames".
+
+;; This two-dimensional nesting approach supports the style of symbolic
+;; execution we do in GL, specifically late binding of free variables in hyps
+;; and RHSes of rules (used for an extension of syntaxp/bind-free).
+
+;; Major stack frames correspond to places in symbolic execution where we enter
+;; an entirely new namespace, such as when we enter the body of a function or
+;; begin relieving the hyps/executing the RHS of a rewrite rule under the
+;; unification substitution.
+
+;; Minor stack frames correspond essentially to entries into lambda bodies.
+;; Except, we process nestings of lambdas into bindinglists (see
+;; centaur/meta/bindinglist) so that if a lambda call is nested directly inside
+;; a lambda body, we reuse the outer frame.  In classical ACL2, each lambda
+;; binds all the variables that are used in its body.  However, when we process
+;; lambdas into bindinglists, we throw out variables that are bound to
+;; themselves, and compensate by appending the new bindings to the existing
+;; bindings.  This helps to support late bindings by allowing us to leave
+;; variables unbound until they are "really used", that is, passed into a
+;; function or bound to a different variable in a lambda.
+
+;; A stack has one or more major stack frames.  A major stack frame has a base
+;; binding list, a debug area, and one or more minor stack frames.  A minor
+;; stack frame has a binding list, a scratch list, and a debug area.
+
+;; The stobj implementation of the stack has three arrays:
+;; - one for minor frames' bindings, scratch, debug fields interleaved
+;; - one for major frames' bindings and debug fields interleaved
+;; - one for the top minor frame pointer of each major frame.
+
+;; A major frame's bottommost minor stack frame is frame 0 for major frame 0,
+;; and the frame after the previous major frame's topmost minor stack frame for
+;; others.
+
+;; The topmost major frame's top minor frame pointer is redundantly recorded in
+;; a top-level field for 1-step access.
 
 
-(fty::defprod stack-frame
+
+(fty::defprod minor-frame
   ((bindings gl-object-alist-p)
    (scratch gl-objectlist-p)
    (debug)))
 
-(fty::deflist stack$a :elt-type stack-frame :true-listp t :non-emptyp t
+(fty::deflist minor-stack :elt-type minor-frame :true-listp t :non-emptyp t
   ///
-  (defthm stack$a-p-of-cons-cdr
-    (implies (and (stack$a-p x)
-                  (stack-frame-p a))
-             (stack$a-p (cons a (cdr x))))
-    :hints(("Goal" :in-theory (enable stack$a-p)))))
+  (defthm minor-stack-p-of-cons-cdr
+    (implies (and (minor-stack-p x)
+                  (minor-frame-p a))
+             (minor-stack-p (cons a (cdr x))))
+    :hints(("Goal" :in-theory (enable minor-stack-p)))))
 
-(define stack$a-push-frame ((x stack$a-p))
-  :enabled t
-  (cons (make-stack-frame) (stack$a-fix x)))
+(make-event
+ `(fty::defprod major-frame
+    ((bindings gl-object-alist-p)
+     (debug)
+     (minor-stack minor-stack-p :default ',(list (make-minor-frame))))))
 
-(define stack$a-len ((x stack$a-p))
+(fty::deflist major-stack :elt-type major-frame :true-listp t :non-emptyp t
+  ///
+  (defthm major-stack-p-of-cons-cdr
+    (implies (and (major-stack-p x)
+                  (major-frame-p a))
+             (major-stack-p (cons a (cdr x))))
+    :hints(("Goal" :in-theory (enable major-stack-p)))))
+
+(define stack$a-frames ((x major-stack-p))
   :enabled t
-  (len x))
+  (len (major-stack-fix x)))
+
+(define stack$a-push-frame ((x major-stack-p))
+  :enabled t
+  (cons (make-major-frame) (major-stack-fix x)))
+
+(define stack$a-minor-frames ((x major-stack-p))
+  :enabled t
+  (len (major-frame->minor-stack (car x))))
+
+(define stack$a-push-minor-frame ((x major-stack-p))
+  :enabled t
+  (b* (((major-frame jframe) (car x)))
+    (major-stack-fix
+     (cons (change-major-frame jframe :minor-stack
+                               (cons (make-minor-frame) jframe.minor-stack))
+           (cdr x)))))
+
+(define stack$a-set-bindings ((bindings gl-object-alist-p)
+                              (x major-stack-p))
+  :enabled t
+  (major-stack-fix (cons (change-major-frame (car x) :bindings bindings)
+                         (cdr x))))
+
+(define stack$a-add-binding ((var pseudo-var-p)
+                             (val gl-object-p)
+                             (x major-stack-p))
+  :enabled t
+  (b* (((major-frame frame) (car x)))
+    (major-stack-fix (cons (change-major-frame frame :bindings (cons (cons (pseudo-var-fix var)
+                                                                           (gl-object-fix val))
+                                                                     frame.bindings))
+                           (cdr x)))))
+
+(define stack$a-set-debug (debug
+                           (x major-stack-p))
+  :enabled t
+  (major-stack-fix (cons (change-major-frame (car x) :debug debug)
+                         (cdr x))))
 
 
 (local (defthm gl-object-alist-p-of-append
@@ -74,443 +167,1271 @@
                          (gl-object-alist-p y))
                     (gl-object-alist-p (append x y)))))
 
-(define stack$a-set-bindings ((bindings gl-object-alist-p)
-                              (x stack$a-p))
+(define stack$a-set-minor-bindings ((bindings gl-object-alist-p)
+                                    (x major-stack-p))
   :enabled t
-  (stack$a-fix (cons (change-stack-frame (car x) :bindings bindings)
-                     (cdr x))))
+  (b* (((major-frame jframe) (car x))
+       (nframe (car jframe.minor-stack)))
+    (major-stack-fix (cons (change-major-frame jframe :minor-stack
+                                               (cons (change-minor-frame nframe :bindings bindings)
+                                                     (cdr jframe.minor-stack)))
+                           (cdr x)))))
 
-(define stack$a-add-bindings ((bindings gl-object-alist-p)
-                              (x stack$a-p))
+(define stack$a-add-minor-bindings ((bindings gl-object-alist-p)
+                                    (x major-stack-p))
   :enabled t
-  (b* (((stack-frame frame) (car x)))
-    (stack$a-fix (cons (change-stack-frame frame :bindings (append bindings frame.bindings))
-                       (cdr x)))))
+  (b* (((major-frame jframe) (car x))
+       ((minor-frame nframe) (car jframe.minor-stack)))
+    (major-stack-fix (cons (change-major-frame jframe :minor-stack
+                                               (cons (change-minor-frame nframe
+                                                                         :bindings (append bindings nframe.bindings))
+                                                     (cdr jframe.minor-stack)))
+                           (cdr x)))))
 
 (define stack$a-push-scratch ((obj gl-object-p)
-                              (x stack$a-p))
+                              (x major-stack-p))
   :enabled t
-  (b* (((stack-frame frame) (car x)))
-    (stack$a-fix (cons (change-stack-frame frame :scratch (cons obj frame.scratch))
-                       (cdr x)))))
+  (b* (((major-frame jframe) (car x))
+       ((minor-frame nframe) (car jframe.minor-stack)))
+    (major-stack-fix (cons (change-major-frame jframe :minor-stack
+                                               (cons (change-minor-frame nframe
+                                                                         :scratch (cons obj nframe.scratch))
+                                                     (cdr jframe.minor-stack)))
+                           (cdr x)))))
 
-(define stack$a-set-debug ((debug)
-                           (x stack$a-p))
+(define stack$a-set-minor-debug ((debug)
+                                 (x major-stack-p))
   :enabled t
-  (b* ((frame (car x)))
-    (stack$a-fix (cons (change-stack-frame frame :debug debug)
-                       (cdr x)))))
+  (b* (((major-frame jframe) (car x))
+       (nframe (car jframe.minor-stack)))
+    (major-stack-fix (cons (change-major-frame jframe :minor-stack
+                                               (cons (change-minor-frame nframe :debug debug)
+                                                     (cdr jframe.minor-stack)))
+                           (cdr x)))))
 
-(define stack$a-bindings ((x stack$a-p))
+(define stack$a-bindings ((x major-stack-p))
   :enabled t
-  (stack-frame->bindings (car x)))
+  (major-frame->bindings (car x)))
 
-(define stack$a-scratchlen ((x stack$a-p))
+(define stack$a-minor-bindings ((x major-stack-p))
   :enabled t
-  (len (stack-frame->scratch (car x))))
+  (minor-frame->bindings (car (major-frame->minor-stack (car x)))))
 
-
-(define revappend-take ((n natp) (x true-listp) acc)
-  (if (zp n)
-      acc
-    (revappend-take (1- n) (cdr x) (cons (car x) acc)))
-  ///
-  (defthm revappend-take-elim
-    (equal (revappend-take n x acc)
-           (revappend (take n x) acc))))
-
-(define rev-take ((n natp) (x true-listp))
-  :inline t
-  (revappend-take n x nil)
-  ///
-  (defthm rev-take-elim
-    (equal (rev-take n x)
-           (rev (take n x)))))
-
-(define stack$a-peek-scratch ((n natp)
-                              (x stack$a-p))
-  :guard (<= n (stack$a-scratchlen x))
+(define stack$a-debug ((x major-stack-p))
   :enabled t
-  (b* (((stack-frame frame) (car x)))
-    (rev-take n frame.scratch)))
+  (major-frame->debug (car x)))
+
+(define stack$a-minor-debug ((x major-stack-p))
+  :enabled t
+  (minor-frame->debug (car (major-frame->minor-stack (car x)))))
+
+(define stack$a-scratchlen ((x major-stack-p))
+  :enabled t
+  (len (minor-frame->scratch (car (major-frame->minor-stack (car x))))))
 
 
 (define stack$a-pop-scratch ((n natp)
-                             (x stack$a-p))
+                             (x major-stack-p))
   :guard (<= n (stack$a-scratchlen x))
   :enabled t
-  (b* (((stack-frame frame) (car x)))
-    (stack$a-fix (cons (change-stack-frame frame :scratch (nthcdr n frame.scratch))
-                       (cdr x)))))
+  (b* (((major-frame jframe) (car x))
+       ((minor-frame nframe) (car jframe.minor-stack)))
+    (major-stack-fix (cons (change-major-frame jframe :minor-stack
+                                               (cons (change-minor-frame nframe
+                                                                         :scratch
+                                                                         (nthcdr n nframe.scratch))
+                                                     (cdr jframe.minor-stack)))
+                           (cdr x)))))
 
-(local
- (defthm stack-frame-p-of-nth-when-stack$a-p
-   (implies (and (stack$a-p x)
-                 (< (nfix n) (len x)))
-            (stack-frame-p (nth n x)))
-   :hints(("Goal" :in-theory (enable stack$a-p nth)))))
-
-(define stack$a-nth-frame ((n natp)
-                           (x stack$a-p))
-  ;; for debugging mostly
+(define stack$a-scratch ((x major-stack-p))
   :enabled t
-  :guard (< n (stack$a-len x))
-  (stack-frame-fix (nth n x)))
+  (minor-frame->scratch (car (major-frame->minor-stack (car x)))))
 
-(defthm stack$a-p-of-cdr
-  (implies (and (stack$a-p x)
-                (< 1 (len x)))
-           (stack$a-p (cdr x)))
-  :hints(("Goal" :in-theory (enable stack$a-p))))
-                  
-       
-(define stack$a-pop-frame ((x stack$a-p))
+(local (defthm len-gt-0
+         (equal (< 0 (len x))
+                (consp x))))
+
+(local (defthm <-cancel
+         (implies (syntaxp (and (quotep c1) (quotep c2)))
+                  (equal (< c1 (+ c2 x))
+                         (< (- c1 c2) (fix x))))
+         :hints (("goal" :Cases ((< c1 (+ c2 x)))))))
+
+(define stack$a-pop-minor-frame ((x major-stack-p))
   :enabled t
-  :guard (< 1 (stack$a-len x))
-  (stack$a-fix (cdr x)))
+  :guard (< 1 (stack$a-minor-frames x))
+  (b* (((major-frame jframe) (car x)))
+    (major-stack-fix (cons (change-major-frame jframe :minor-stack (cdr jframe.minor-stack))
+                           (cdr x)))))
+
+(define stack$a-pop-frame ((x major-stack-p))
+  :enabled t
+  :guard (and (< 1 (stack$a-frames x))
+              (eql 1 (stack$a-minor-frames x)))
+  (major-stack-fix (cdr x)))
+
+(define stack$a-extract ((x major-stack-p))
+  :enabled t
+  (major-stack-fix x))
 
 (define create-stack$a ()
   :enabled t
-  (list (make-stack-frame)))
+  (list (make-major-frame)))
+
+;; (local
+;;  (defthm major-frame-p-of-nth-when-major-stack-p
+;;    (implies (and (major-stack-p x)
+;;                  (< (nfix n) (len x)))
+;;             (major-frame-p (nth n x)))
+;;    :hints(("Goal" :in-theory (enable major-stack-p nth)))))
+
+;; (local
+;;  (defthm minor-frame-p-of-nth-when-minor-stack-p
+;;    (implies (and (minor-stack-p x)
+;;                  (< (nfix n) (len x)))
+;;             (minor-frame-p (nth n x)))
+;;    :hints(("Goal" :in-theory (enable minor-stack-p nth)))))
+
+;; (define stack$a-nth-frame ((n natp)
+;;                            (x major-stack-p))
+;;   ;; for debugging mostly
+;;   :enabled t
+;;   :guard (< n (stack$a-len x))
+;;   (stack-frame-fix (nth n x)))
+
+;; (defthm major-stack-p-of-cdr
+;;   (implies (and (major-stack-p x)
+;;                 (< 1 (len x)))
+;;            (major-stack-p (cdr x)))
+;;   :hints(("Goal" :in-theory (enable major-stack-p))))
+                  
+       
+;; (define major-stack-pop-frame ((x major-stack-p))
+;;   :enabled t
+;;   :guard (< 1 (stack$a-len x))
+;;   (major-stack-fix (cdr x)))
 
 
+(local (defthm nfix-when-natp
+         (implies (natp n)
+                  (equal (nfix n) n))))
+
+(local (defthm max-greater-equal-1
+         (<= a (max a b))
+         :rule-classes :linear))
+(local (defthm max-greater-equal-2
+         (<= b (max a b))
+         :rule-classes :linear))
+(local (in-theory (disable not max nfix natp len resize-list)))
+
+(local (std::remove-default-post-define-hook :fix))
 
 (defstobj stack$c
-  (stack$c-array :type (array t (3)) :resizable t)
-  (stack$c-nframes :type (integer 1 *) :initially 1))
+  (stack$c-minor :type (array t (3)) :resizable t)
+  (stack$c-major :type (array t (2)) :resizable t)
+  (stack$c-top-minor :type (array (unsigned-byte 32) (1)) :resizable t :initially 0)
+  (stack$c-top-frame :type (unsigned-byte 32) :initially 0)
+  (stack$c-top-minor-frame :type (unsigned-byte 32) :initially 0)
+  :renaming ((stack$c-top-minori stack$c-top-minori1)
+             (stack$c-top-frame stack$c-top-frame1)
+             (stack$c-top-minor-frame stack$c-top-minor-frame1)))
 
 
-(defun-sk stack$c-welltyped (stack$c)
+
+(define nth-nat ((n natp) (x true-listp))
+  :returns (val natp :rule-classes :type-prescription)
+  (nfix (nth n x))
+  ///
+  (defthm nth-nat-of-update-nth
+    (equal (nth-nat m (update-nth n val l))
+           (if (equal (nfix m) (nfix n))
+               (nfix val)
+             (nth-nat m l))))
+
+  (fty::deffixequiv nth-nat))
+
+
+(define stack$c-top-minori ((i natp :type (integer 0 *))
+                            (stack$c))
+  :guard (< i (stack$c-top-minor-length stack$c))
+  :split-types t
+  :enabled t
+  :inline t
+  :guard-hints (("goal" :in-theory (enable nth-nat)))
+  :prepwork ((local
+              (defthm stack$c-top-minorp-implies-natp-nth
+                (implies (and (stack$c-top-minorp x)
+                              (< (nfix n) (len x)))
+                         (natp (nth n x)))
+                :hints(("Goal" :in-theory (enable nth len)))
+                :rule-classes (:rewrite (:type-prescription :typed-term (nth n x))))))
+  (mbe :logic (non-exec (nth-nat i (nth *stack$c-top-minori1* stack$c)))
+       :exec (stack$c-top-minori1 i stack$c)))
+
+(define stack$c-top-frame ((stack$c))
+  :enabled t
+  :inline t
+  :guard-hints (("goal" :in-theory (enable nth-nat)))
+  (mbe :logic (nth-nat *stack$c-top-frame1* (non-exec stack$c))
+       :exec (stack$c-top-frame1 stack$c)))
+
+(define stack$c-top-minor-frame ((stack$c))
+  :enabled t
+  :inline t
+  :guard-hints (("goal" :in-theory (enable nth-nat)))
+  (mbe :logic (nth-nat *stack$c-top-minor-frame1* (non-exec stack$c))
+       :exec (stack$c-top-minor-frame1 stack$c)))
+
+(defun-sk stack$c-minor-frames-welltyped (stack$c)
   (forall i
           (implies (natp i)
-                   (and (gl-object-alist-p (nth (* 3 i) (nth *stack$c-arrayi* stack$c)))
-                        (gl-objectlist-p (nth (+ 1 (* 3 i)) (nth *stack$c-arrayi* stack$c))))))
+                   (and (gl-object-alist-p (nth (* 3 i) (nth *stack$c-minori* stack$c)))
+                        (gl-objectlist-p (nth (+ 1 (* 3 i)) (nth *stack$c-minori* stack$c))))))
   :rewrite :direct)
 
-(in-theory (disable stack$c-welltyped))
+(in-theory (disable stack$c-minor-frames-welltyped
+                    stack$c-minor-frames-welltyped-necc))
 
-(defthm stack$c-welltyped-implies-gl-object-alist-p
-  (implies (and (stack$c-welltyped stack$c)
-                (posp n) (<= n (stack$c-nframes stack$c)))
-           (gl-object-alist-p (nth (+ -3 (* 3 n)) (nth *stack$c-arrayi* stack$c))))
-  :hints (("goal" :use ((:instance stack$c-welltyped-necc (i (1- n))))
-           :in-theory (disable stack$c-welltyped-necc))))
+(local (in-theory (enable stack$c-minor-frames-welltyped-necc)))
 
-(defthm stack$c-welltyped-implies-gl-objectlist-p
-  (implies (and (stack$c-welltyped stack$c)
-                (posp n) (<= n (stack$c-nframes stack$c)))
-           (gl-objectlist-p (nth (+ -2 (* 3 n)) (nth *stack$c-arrayi* stack$c))))
-  :hints (("goal" :use ((:instance stack$c-welltyped-necc (i (1- n))))
-           :in-theory (disable stack$c-welltyped-necc))))
+(local
+ (defthm stack$c-minor-frames-welltyped-zero
+   (implies (stack$c-minor-frames-welltyped stack$c)
+            (and (gl-object-alist-p (nth 0 (nth *stack$c-minori* stack$c)))
+                 (gl-objectlist-p (nth 1 (nth *stack$c-minori* stack$c)))))
+   :hints (("goal" :use ((:instance stack$c-minor-frames-welltyped-necc (i 0)))))))
 
-(defun-sk stack$c-bounded (stack$c)
-  ;; Elements outside the frames are all set to 0.
+;; (defthm stack$c-minor-frames-welltyped-implies-gl-object-alist-p
+;;   (implies (and (stack$c-minor-frames-welltyped stack$c)
+;;                 (posp n) (<= n (stack$c-nframes stack$c)))
+;;            (gl-object-alist-p (nth (+ -3 (* 3 n)) (nth *stack$c-minori* stack$c))))
+;;   :hints (("goal" :use ((:instance stack$c-minor-frames-welltyped-necc (i (1- n))))
+;;            :in-theory (disable stack$c-minor-frames-welltyped-necc))))
+
+;; (defthm stack$c-minor-frames-welltyped-implies-gl-objectlist-p
+;;   (implies (and (stack$c-minor-frames-welltyped stack$c)
+;;                 (posp n) (<= n (stack$c-nframes stack$c)))
+;;            (gl-objectlist-p (nth (+ -2 (* 3 n)) (nth *stack$c-minori* stack$c))))
+;;   :hints (("goal" :use ((:instance stack$c-minor-frames-welltyped-necc (i (1- n))))
+;;            :in-theory (disable stack$c-minor-frames-welltyped-necc))))
+
+(defun-sk stack$c-major-frames-welltyped (stack$c)
+  (forall i
+          (implies (natp i)
+                   (gl-object-alist-p (nth (* 2 i) (nth *stack$c-majori* stack$c)))))
+  :rewrite :direct)
+
+(in-theory (disable stack$c-major-frames-welltyped
+                    stack$c-major-frames-welltyped-necc))
+
+(local (in-theory (enable stack$c-major-frames-welltyped-necc)))
+
+(local
+ (defthm stack$c-major-frames-welltyped-zero
+   (implies (stack$c-major-frames-welltyped stack$c)
+            (gl-object-alist-p (nth 0 (nth *stack$c-majori* stack$c))))
+   :hints (("goal" :use ((:instance stack$c-major-frames-welltyped-necc (i 0)))))))
+
+
+(defun-sk stack$c-top-minor-ordered (stack$c)
+  (forall (i j)
+          (implies (and (natp i)
+                        (integerp j)
+                        (< i j)
+                        (<= j (stack$c-top-frame stack$c)))
+                   (< (nth-nat i (nth *stack$c-top-minori1* stack$c))
+                      (nth-nat j (nth *stack$c-top-minori1* stack$c)))))
+  :rewrite :direct)
+
+(in-theory (disable stack$c-top-minor-ordered
+                    stack$c-top-minor-ordered-necc))
+
+(local (in-theory (enable stack$c-top-minor-ordered-necc)))
+
+(local
+ (defthm stack$c-top-minor-ordered-lte
+   (implies (and (stack$c-top-minor-ordered stack$c)
+                 (natp i)
+                 (integerp j)
+                 (<= i j)
+                 (<= j (stack$c-top-frame stack$c)))
+            (and (<= (nth-nat i (nth *stack$c-top-minori1* stack$c))
+                     (nth-nat j (nth *stack$c-top-minori1* stack$c)))
+                 (< (nth-nat i (nth *stack$c-top-minori1* stack$c))
+                    (+ 1 (nth-nat j (nth *stack$c-top-minori1* stack$c))))))
+   :hints (("goal" :use ((:instance stack$c-top-minor-ordered-necc))
+            :in-theory (disable stack$c-top-minor-ordered-necc)))))
+
+(local
+ (defthm stack$c-top-minor-ordered-minus1
+   (implies (and (stack$c-top-minor-ordered stack$c)
+                 (posp i)
+                 (<= i (stack$c-top-frame stack$c)))
+            (and (< (nth-nat (+ -1 i) (nth *stack$c-top-minori1* stack$c))
+                    (nth-nat i (nth *stack$c-top-minori1* stack$c)))
+                 (<= (+ 1 (nth-nat (+ -1 i) (nth *stack$c-top-minori1* stack$c)))
+                     (nth-nat i (nth *stack$c-top-minori1* stack$c)))))
+   :hints (("goal" :use ((:instance stack$c-top-minor-ordered-necc (i (+ -1 i)) (j i)))
+            :in-theory (disable stack$c-top-minor-ordered-necc)))
+   :rule-classes (:rewrite :linear)))
+
+(local
+ (defthm stack$c-top-minor-ordered-plus1
+   (implies (and (stack$c-top-minor-ordered stack$c)
+                 (natp i)
+                 (< i (stack$c-top-frame stack$c)))
+            (and (< (nth-nat i (nth *stack$c-top-minori1* stack$c))
+                    (nth-nat (+ 1 i) (nth *stack$c-top-minori1* stack$c)))
+                 (<= (+ 1 (nth-nat i (nth *stack$c-top-minori1* stack$c)))
+                     (nth-nat (+ 1 i) (nth *stack$c-top-minori1* stack$c)))))
+   :hints (("goal" :use ((:instance stack$c-top-minor-ordered-necc (i i) (j (+ 1 i))))
+            :in-theory (disable stack$c-top-minor-ordered-necc)))
+   :rule-classes (:rewrite :linear)))
+
+
+(defun-sk stack$c-minor-frames-bounded (stack$c)
   (forall i
           (implies (and (natp i)
-                        (<= (* 3 (stack$c-nframes stack$c)) i))
-                   (equal (nth i (nth *stack$c-arrayi* stack$c)) nil)))
+                        (<= (+ 3 (* 3 (nth-nat (stack$c-top-frame stack$c)
+                                               (nth *stack$c-top-minori1* stack$c))))
+                            i))
+                   (equal (nth i (nth *stack$c-minori* stack$c)) nil)))
   :rewrite :direct)
 
-(in-theory (disable stack$c-bounded))
+(in-theory (disable stack$c-minor-frames-bounded
+                    stack$c-minor-frames-bounded-necc))
+
+(local (in-theory (enable stack$c-minor-frames-bounded-necc)))
+
+(defun-sk stack$c-major-frames-bounded (stack$c)
+  (forall i
+          (implies (and (natp i)
+                        (<= (+ 2 (* 2 (stack$c-top-frame stack$c)))
+                            i))
+                   (equal (nth i (nth *stack$c-majori* stack$c)) nil)))
+  :rewrite :direct)
+
+(in-theory (disable stack$c-major-frames-bounded
+                    stack$c-major-frames-bounded-necc))
+
+(local (in-theory (enable stack$c-major-frames-bounded-necc)))
+
+
 
 (define stack$c-okp (stack$c)
   :enabled t
-  (and (<= (* 3 (stack$c-nframes stack$c)) (stack$c-array-length stack$c))
-       (ec-call (stack$c-welltyped stack$c))
-       (ec-call (stack$c-bounded stack$c))))
+  (and (<= (+ 2 (* 2 (stack$c-top-frame stack$c))) (stack$c-major-length stack$c))
+       (<= (+ 1 (stack$c-top-frame stack$c)) (stack$c-top-minor-length stack$c))
+       (<= (+ 3 (* 3 (stack$c-top-minori (stack$c-top-frame stack$c) stack$c)))
+           (stack$c-minor-length stack$c))
+       (equal (stack$c-top-minor-frame stack$c)
+              (stack$c-top-minori (stack$c-top-frame stack$c) stack$c))
+       (ec-call (stack$c-top-minor-ordered stack$c))
+       (ec-call (stack$c-major-frames-welltyped stack$c))
+       (ec-call (stack$c-minor-frames-welltyped stack$c))
+       (ec-call (stack$c-major-frames-bounded stack$c))
+       (ec-call (stack$c-minor-frames-bounded stack$c))))
 
-
-
-(define stack$c-push-frame ((stack$c stack$c-okp))
-  :enabled t
-  (b* ((new-len (* 3 (+ 1 (stack$c-nframes stack$c))))
-       (stack$c (if (< (stack$c-array-length stack$c) new-len)
-                    (resize-stack$c-array (max 30 (* 2 new-len)) stack$c)
-                  stack$c)))
-    (update-stack$c-nframes (+ 1 (stack$c-nframes stack$c)) stack$c)))
-
-
-(define stack$c-len (stack$c)
-  :enabled t
-  (stack$c-nframes stack$c))
-
-(define stack$c-set-bindings ((bindings gl-object-alist-p)
-                              (stack$c stack$c-okp))
-  :enabled t
-  (update-stack$c-arrayi (- (* 3 (stack$c-nframes stack$c)) 3) bindings stack$c))
-
-(define stack$c-add-bindings ((bindings gl-object-alist-p)
-                              (stack$c stack$c-okp))
-  :enabled t
-  (b* ((index (- (* 3 (stack$c-nframes stack$c)) 3))
-       (curr-bindings (stack$c-arrayi index stack$c)))
-    (update-stack$c-arrayi index (append bindings curr-bindings) stack$c)))
-
-(define stack$c-push-scratch ((obj gl-object-p)
-                              (stack$c stack$c-okp))
-  :enabled t
-  (b* ((index (- (* 3 (stack$c-nframes stack$c)) 2))
-       (curr-scratch (stack$c-arrayi index stack$c)))
-    (update-stack$c-arrayi index (cons obj curr-scratch) stack$c)))
-
-(define stack$c-set-debug ((obj)
-                           (stack$c stack$c-okp))
-  :enabled t
-  (b* ((index (- (* 3 (stack$c-nframes stack$c)) 1)))
-    (update-stack$c-arrayi index obj stack$c)))
-
-(define stack$c-bindings ((stack$c stack$c-okp))
-  :enabled t
-  (stack$c-arrayi (- (* 3 (stack$c-nframes stack$c)) 3) stack$c))
-
-(define stack$c-scratchlen ((stack$c stack$c-okp))
-  :enabled t
-  (len (stack$c-arrayi (- (* 3 (stack$c-nframes stack$c)) 2) stack$c)))
-
-(local (defthm true-listp-when-gl-objectlist-p-rw
-         (implies (gl-objectlist-p x)
-                  (true-listp x))))
-
-(define stack$c-peek-scratch ((n natp)
-                              (stack$c stack$c-okp))
-  :guard (<= n (stack$c-scratchlen stack$c))
-  :enabled t
-  (rev-take n (stack$c-arrayi (- (* 3 (stack$c-nframes stack$c)) 2) stack$c)))
-
-(define stack$c-pop-scratch ((n natp)
-                             (stack$c stack$c-okp))
-  :guard (<= n (stack$c-scratchlen stack$c))
-  :enabled t
-  (b* ((index (- (* 3 (stack$c-nframes stack$c)) 2)))
-    (update-stack$c-arrayi index (nthcdr n (stack$c-arrayi index stack$c)) stack$c)))
-
-
-;; (local
-;;  (encapsulate nil
-;;    (local (defthm negative-norm
-;;             (equal (- x) (* -1 x))))
-;;    (defthm const-times-negative
-;;      (implies (syntaxp (quotep c))
-;;               (equal (* c (- x))
-;;                      (* (- c) x)))
-;;      :hints (("goal" :use ((:instance associativity-of-*
-;;                             (x -1) (y c) (z x))
-;;                            (:instance associativity-of-*
-;;                             (x c) (y -1) (z x)))
-;;               :in-theory (disable associativity-of-*))))))
-
-
-
-(define stack$c-nth-frame ((n natp)
-                           (stack$c stack$c-okp))
-  :enabled t
-  :guard (< n (stack$c-len stack$c))
-  :guard-hints (("goal" :in-theory (disable distributivity))
-                (and stable-under-simplificationp
-                     '(:in-theory (enable distributivity))))
-  :prepwork ((local
-              (encapsulate nil
-                (defthm <-when-<=
-                  (implies (and (<= a b)
-                                (< c 0)
-                                (<= d 0))
-                           (< (+ c d a) b)))
-
-                (local (defthmd foo1
-                         (implies (and (integerp i)
-                                       (< i 0)
-                                       (<= -3 i)
-                                       (posp m))
-                                  (<= 0 (+ i (* 3 m))))))
-
-                (defthm foo
-                  (implies (and (integerp i)
-                                (< i 0)
-                                (<= -3 i)
-                                (integerp n)
-                                (natp m)
-                                (< n m))
-                           (<= 0 (+ i (* 3 (- n)) (* 3 m))))
-                  :hints (("goal" :use ((:instance foo1 (m (- m n))))))))))
-  (b* ((offset (* 3 (- (stack$c-len stack$c) n))))
-    (make-stack-frame :bindings (stack$c-arrayi (- offset 3) stack$c)
-                      :scratch (stack$c-arrayi (- offset 2) stack$c)
-                      :debug (stack$c-arrayi (- offset 1) stack$c))))
-
-(define stack$c-pop-frame ((stack$c stack$c-okp))
-  :guard (< 1 (stack$c-len stack$c))
-  :enabled t
-  (b* ((offset (* 3 (stack$c-nframes stack$c)))
-       (stack$c (update-stack$c-arrayi (- offset 1) nil stack$c))
-       (stack$c (update-stack$c-arrayi (- offset 2) nil stack$c))
-       (stack$c (update-stack$c-arrayi (- offset 3) nil stack$c)))
-    (update-stack$c-nframes (1- (stack$c-nframes stack$c)) stack$c)))
-
-(encapsulate nil
-  (local (defun-sk stack-frames-corr (stack$c stack$a)
-           (forall n
-                   (implies (and (natp n)
-                                 (< n (len stack$a)))
-                            (and (equal (nth (* 3 n) (nth *stack$c-arrayi* stack$c))
-                                        (stack-frame->bindings (nth (- (+ -1 (len stack$a)) n) stack$a)))
-                                 (equal (nth (+ 1 (* 3 n)) (nth *stack$c-arrayi* stack$c))
-                                        (stack-frame->scratch (nth (- (+ -1 (len stack$a)) n) stack$a)))
-                                 (equal (nth (+ 2 (* 3 n)) (nth *stack$c-arrayi* stack$c))
-                                        (stack-frame->debug (nth (- (+ -1 (len stack$a)) n) stack$a))))))
-           :rewrite :direct))
-  (local (in-theory (disable stack-frames-corr)))
-
-  (local (defthm stack-frames-corr-offset
-           (implies (and (stack-frames-corr stack$c stack$a)
-                         (posp n)
-                         (<= n (len stack$a)))
-                    (and (equal (nth (+ -3 (* 3 n)) (nth *stack$c-arrayi* stack$c))
-                                (stack-frame->bindings (nth (- (len stack$a) n) stack$a)))
-                         (equal (nth (+ -2 (* 3 n)) (nth *stack$c-arrayi* stack$c))
-                                (stack-frame->scratch (nth (- (len stack$a) n) stack$a)))
-                         (equal (nth (+ -1 (* 3 n)) (nth *stack$c-arrayi* stack$c))
-                                (stack-frame->debug (nth (- (len stack$a) n) stack$a)))))
-           :hints (("goal" :use ((:instance stack-frames-corr-necc (n (1- n))))
-                    :in-theory (disable stack-frames-corr-necc)))))
-
-  (local (defthm stack-frames-corr-offset2
-           (implies (and (stack-frames-corr stack$c stack$a)
-                         (integerp m) (integerp n)
-                         (posp (+ n m))
-                         (<= (+ n m) (len stack$a)))
-                    (and (equal (nth (+ -3 (* 3 n) (* 3 m)) (nth *stack$c-arrayi* stack$c))
-                                (stack-frame->bindings (nth (- (len stack$a) (+ n m)) stack$a)))
-                         (equal (nth (+ -2 (* 3 n) (* 3 m)) (nth *stack$c-arrayi* stack$c))
-                                (stack-frame->scratch (nth (- (len stack$a) (+ n m)) stack$a)))
-                         (equal (nth (+ -1 (* 3 n) (* 3 m)) (nth *stack$c-arrayi* stack$c))
-                                (stack-frame->debug (nth (- (len stack$a) (+ n m)) stack$a)))))
-           :hints (("goal" :use ((:instance stack-frames-corr-necc (n (1- (+ n m)))))
-                    :in-theory (disable stack-frames-corr-necc)))))
-
-  (local (defthm stack-frames-corr-zero-offset
-           (implies (and (stack-frames-corr stack$c stack$a)
-                         (integerp m) (integerp n)
-                         (posp (+ n m))
-                         (<= (+ n m) (len stack$a)))
-                    (and (equal (nth 0 (nth *stack$c-arrayi* stack$c))
-                                (stack-frame->bindings (nth (- (len stack$a) 1) stack$a)))
-                         (equal (nth 1 (nth *stack$c-arrayi* stack$c))
-                                (stack-frame->scratch (nth (- (len stack$a) 1) stack$a)))
-                         (equal (nth 2 (nth *stack$c-arrayi* stack$c))
-                                (stack-frame->debug (nth (- (len stack$a) 1) stack$a)))))
-           :hints (("goal" :use ((:instance stack-frames-corr-necc (n 0)))
-                    :in-theory (disable stack-frames-corr-necc)))))
-
-  (local (define stack-corr (stack$c stack$a)
-           :non-executable t
-           :enabled t
-           (and (stack$c-okp stack$c)
-                (equal (stack$c-nframes stack$c) (len stack$a))
-                (ec-call (stack-frames-corr stack$c stack$a)))))
-
-  ;; (local (defthm nth-of-cons-when-zp
-  ;;          (implies (zp n)
-  ;;                   (equal (nth n (cons a b))
-  ;;                          a))
-  ;;          :hints(("Goal" :in-theory (enable nth)))))
-
-  ;; (local (defthm nth-of-cons-when-posp
-  ;;          (implies (posp n)
-  ;;                   (equal (nth n (cons a b))
-  ;;                          (nth (+ -1 n) b)))
-  ;;          :hints(("Goal" :in-theory (enable nth)))))
-
-  (local (defthm nth-of-cons-split
+(local
+ (encapsulate nil
+   (local (defthm nth-of-cons-split
            (equal (nth n (cons a b))
                   (if (zp n)
                       a
                     (nth (+ -1 n) b)))
            :hints(("Goal" :in-theory (enable nth)))))
+   (defthm stack$c-okp-of-create-stack$c
+         (stack$c-okp (create-stack$c))
+         :hints(("Goal" :in-theory (enable stack$c-major-frames-welltyped
+                                           stack$c-minor-frames-welltyped
+                                           stack$c-major-frames-bounded
+                                           stack$c-minor-frames-bounded
+                                           stack$c-top-minor-ordered
+                                           nth))))))
 
+(define stack$c-frames ((stack$c stack$c-okp))
+  :enabled t
+  (lposfix (+ 1 (stack$c-top-frame stack$c))))
+
+
+(define maybe-grow-list ((threshold natp)
+                         (default)
+                         (list))
+  :verify-guards nil
+  :returns (new-list)
+  (if (< (len list) (lnfix threshold))
+      (resize-list list (max 16 (* 2 (lnfix threshold))) default)
+    list)
+  ///
+  (defret len-of-maybe-grow-list-grows
+    (<= (len list) (len new-list))
+    :rule-classes :linear)
+
+  (defret len-of-maybe-grow-list-sufficient
+    (<= (nfix threshold) (len new-list))
+    :rule-classes :linear)
+
+  (defret nth-of-maybe-grow-list-under
+    (implies (< (nfix n) (len list))
+             (equal (nth n new-list) (nth n list))))
+
+  (defthm nth-of-maybe-grow-list-when-default-nil
+    (let ((new-list (maybe-grow-list threshold nil list)))
+      (equal (nth n new-list) (nth n list))))
+
+  (defthm nth-nat-of-maybe-grow-list
+    (let ((new-list (maybe-grow-list threshold 0 list)))
+      (equal (nth-nat n new-list) (nth-nat n list)))
+    :hints(("Goal" :in-theory (enable nth-nat)))))
+
+(local (defthmd update-nth-redundant-free
+         (implies (and (equal val (nth n x))
+                       (< (nfix n) (len x)))
+                  (equal (update-nth n val x) x))
+         :hints(("Goal" :in-theory (enable nth update-nth len)))))
+
+(define stack$c-push-frame ((stack$c stack$c-okp))
+  :enabled t
+  :guard-hints ((and stable-under-simplificationp
+                     '(:in-theory (enable maybe-grow-list
+                                          update-nth-redundant-free))))
   
-
-  (local (defthm equal-plus-consts
-           (implies (syntaxp (and (quotep a) (quotep b)))
-                    (equal (equal (+ a c) (+ b d))
-                           (equal (+ (+ (- b) a) c) (fix d))))))
-
-  (local (defthm equal-const-plus-3*
-           (implies (syntaxp (quotep c))
-                    (equal (equal (+ c (* 3 x)) (* 3 y))
-                           (equal (+ (/ c 3) x) (fix y))))))
-
-  
-  (local (defthm len-cons
-           (equal (len (cons a b))
-                  (+ 1 (len b)))))
-
-  (local (defthm nfix-when-natp
-           (implies (natp n)
-                    (equal (nfix n) n))))
-
-  (local (defthm natp-when-integerp-gte-0
-           (implies (and (integerp x)
-                         (<= 0 x))
-                    (natp x))))
-
-
-  (local (defthm <=-max
-           (implies (or (<= x a) (<= x b))
-                    (<= x (max a b)))))
-
-  (local (defthm <-max
-           (implies (or (< x a) (< x b))
-                    (< x (max a b)))))
-
-  (local (defthm minus-minus
-           (equal (- (- x)) (fix x))))
-
-  (local (in-theory (disable len nfix not natp max
-                             acl2::nth-when-atom
-                             true-listp-update-nth
-                             acl2::nth-when-too-large-cheap
-                             resize-list nthcdr acl2::take-redefinition
-                             append
-                             acl2::nthcdr-when-zp)))
-
-  (local (defthm len-when-stack$a-p
-           (implies (stack$a-p x)
-                    (posp (len x)))
-           :hints(("Goal" :in-theory (enable stack$a-p)))
-           :rule-classes :forward-chaining))
-
-
-  (local (set-default-hints
-          '((and stable-under-simplificationp
-                 (let ((lit (car (last clause))))
-                   (and (or (eq (car lit) 'stack$c-welltyped)
-                            (eq (car lit) 'stack$c-bounded)
-                            (eq (car lit) 'stack-frames-corr))
-                        `(:expand (,lit)))))
-            ;; (and stable-under-simplificationp
-            ;;      '(:in-theory (enable nth-of-cons-split)))
-            )))
-                             
-  (defabsstobj-events stack
-    :concrete stack$c
-    :corr-fn stack-corr
-    :recognizer (stackp :logic stack$a-p
-                        :exec stack$cp)
-    :creator (create-stack :logic create-stack$a
-                           :exec create-stack$c)
-    :exports ((stack-push-frame :logic stack$a-push-frame :exec stack$c-push-frame :protect t)
-              (stack-len :logic stack$a-len :exec stack$c-len)
-              (stack-set-bindings :logic stack$a-set-bindings :exec stack$c-set-bindings)
-              (stack-add-bindings :logic stack$a-add-bindings :exec stack$c-add-bindings)
-              (stack-push-scratch :logic stack$a-push-scratch :exec stack$c-push-scratch)
-              (stack-set-debug :logic stack$a-set-debug :exec stack$c-set-debug)
-              (stack-bindings :logic stack$a-bindings :exec stack$c-bindings)
-              (stack-scratchlen :logic stack$a-scratchlen :exec stack$c-scratchlen)
-              (stack-peek-scratch :logic stack$a-peek-scratch :exec stack$c-peek-scratch)
-              (stack-pop-scratch :logic stack$a-pop-scratch :exec stack$c-pop-scratch)
-              (stack-nth-frame :logic stack$a-nth-frame :exec stack$c-nth-frame)
-              (stack-pop-frame :logic stack$a-pop-frame :exec stack$c-pop-frame :protect t)
-              )))
-
-
+  (b* ((prev-top-major (stack$c-top-frame stack$c))
+       (new-major-len (+ 4 (* 2 prev-top-major)))
+       (stack$c (mbe :logic (non-exec (update-nth *stack$c-majori*
+                                                  (maybe-grow-list
+                                                   new-major-len nil
+                                                   (nth *stack$c-majori* stack$c))
+                                                  stack$c))
+                     :exec (if (< (stack$c-major-length stack$c) new-major-len)
+                               (resize-stack$c-major (max 16 (* 2 new-major-len)) stack$c)
+                             stack$c)))
+       (new-top-len (+ 2 prev-top-major))
+       (stack$c (mbe :logic (non-exec (update-nth *stack$c-top-minori1*
+                                                  (maybe-grow-list
+                                                   new-top-len 0
+                                                   (nth *stack$c-top-minori1* stack$c))
+                                                  stack$c))
+                     :exec (if (< (stack$c-top-minor-length stack$c) new-top-len)
+                               (resize-stack$c-top-minor (max 16 (* 2 new-top-len)) stack$c)
+                             stack$c)))
+       (prev-top-minor (stack$c-top-minor-frame stack$c))
+       (new-minor-len (+ 6 (* 3 prev-top-minor)))
+       (stack$c (mbe :logic (non-exec (update-nth *stack$c-minori*
+                                                  (maybe-grow-list
+                                                   new-minor-len nil
+                                                   (nth *stack$c-minori* stack$c))
+                                                  stack$c))
+                     :exec (if (< (stack$c-minor-length stack$c) new-minor-len)
+                               (resize-stack$c-minor (max 16 (* 2 new-minor-len)) stack$c)
+                             stack$c)))
+       (new-top-minor (+ 1 prev-top-minor))
+       (stack$c (mbe :logic (b* ((stack$c (update-stack$c-top-minori (+ 1 prev-top-major) new-top-minor stack$c)))
+                              (update-stack$c-top-minor-frame new-top-minor stack$c))
+                     :exec (if (<= new-top-minor #xffffffff)
+                               (b* ((stack$c (update-stack$c-top-minori (+ 1 prev-top-major) new-top-minor stack$c)))
+                                 (update-stack$c-top-minor-frame new-top-minor stack$c))
+                             (b* ((stack$c (ec-call (update-stack$c-top-minori (+ 1 prev-top-major) new-top-minor stack$c))))
+                               (ec-call (update-stack$c-top-minor-frame new-top-minor stack$c))))))
+       (new-top-major (+ 1 prev-top-major)))
+    (mbe :logic (update-stack$c-top-frame new-top-major stack$c)
+         :exec (if (<= new-top-major #xffffffff)
+                   (update-stack$c-top-frame new-top-major stack$c)
+                 (ec-call (update-stack$c-top-frame new-top-major stack$c))))))
        
+(define stack$c-minor-frames ((stack$c stack$c-okp))
+  :enabled t
+  (b* ((top-major (stack$c-top-frame stack$c))
+       (top-minor (stack$c-top-minori top-major stack$c))
+       (prev-top-minor (if (eql 0 top-major)
+                           -1
+                         (stack$c-top-minori (+ -1 top-major) stack$c))))
+    (- top-minor prev-top-minor)))
+
+(define stack$c-push-minor-frame ((stack$c stack$c-okp))
+  :enabled t
+  :guard-hints ((and stable-under-simplificationp
+                     '(:in-theory (enable maybe-grow-list
+                                          update-nth-redundant-free))))
+  
+  (b* ((top-major (stack$c-top-frame stack$c))
+       (top-minor (stack$c-top-minor-frame stack$c))
+       (new-top-minor (+ 1 top-minor))
+       (new-minor-len (+ 3 (* 3 new-top-minor)))
+       (stack$c (mbe :logic (non-exec (update-nth *stack$c-minori*
+                                                  (maybe-grow-list
+                                                   new-minor-len nil
+                                                   (nth *stack$c-minori* stack$c))
+                                                  stack$c))
+                     :exec (if (< (stack$c-minor-length stack$c) new-minor-len)
+                               (resize-stack$c-minor (max 16 (* 2 new-minor-len)) stack$c)
+                             stack$c))))
+    (mbe :logic
+         (b* ((stack$c (update-stack$c-top-minori top-major new-top-minor stack$c)))
+           (update-stack$c-top-minor-frame new-top-minor stack$c))
+         :exec
+         (if (<= new-top-minor #xffffffff)
+             (b* ((stack$c (update-stack$c-top-minori top-major new-top-minor stack$c)))
+               (update-stack$c-top-minor-frame new-top-minor stack$c))
+           (b* ((stack$c (ec-call (update-stack$c-top-minori top-major new-top-minor stack$c))))
+             (ec-call (update-stack$c-top-minor-frame new-top-minor stack$c)))))))
+       
+(define stack$c-set-bindings ((bindings gl-object-alist-p)
+                              (stack$c stack$c-okp))
+  :enabled t
+  (b* ((top-major (stack$c-top-frame stack$c)))
+    (update-stack$c-majori (* 2 top-major) bindings stack$c)))
+       
+
+(define stack$c-add-binding ((var pseudo-var-p)
+                             (val gl-object-p)
+                             (stack$c stack$c-okp))
+  :enabled t
+  (b* ((top-major (stack$c-top-frame stack$c))
+       (index (* 2 top-major)))
+    (update-stack$c-majori index (cons (cons var val) (stack$c-majori index stack$c))
+                           stack$c)))
+
+(define stack$c-set-debug (debug
+                           (stack$c stack$c-okp))
+  :enabled t
+  (b* ((top-major (stack$c-top-frame stack$c)))
+    (update-stack$c-majori (+ 1 (* 2 top-major)) debug stack$c)))
+
+(define stack$c-set-minor-bindings ((bindings gl-object-alist-p)
+                                    (stack$c stack$c-okp))
+  :enabled t
+  :guard-hints (("goal" :do-not-induct t))
+  (b* ((top-minor (stack$c-top-minor-frame stack$c)))
+    (update-stack$c-minori (* 3 top-minor) bindings stack$c)))
+
+(define stack$c-add-minor-bindings ((bindings gl-object-alist-p)
+                                    (stack$c stack$c-okp))
+  :enabled t
+  (b* ((top-minor (stack$c-top-minor-frame stack$c))
+       (index (* 3 top-minor)))
+    (update-stack$c-minori index
+                           (append bindings (stack$c-minori index stack$c))
+                           stack$c)))
+
+(define stack$c-push-scratch ((obj gl-object-p)
+                              (stack$c stack$c-okp))
+  :enabled t
+  (b* ((top-minor (stack$c-top-minor-frame stack$c))
+       (index (+ 1 (* 3 top-minor))))
+    (update-stack$c-minori index
+                           (cons obj (stack$c-minori index stack$c))
+                           stack$c)))
+
+(define stack$c-set-minor-debug ((debug)
+                                 (stack$c stack$c-okp))
+  :enabled t
+  (b* ((top-minor (stack$c-top-minor-frame stack$c)))
+    (update-stack$c-minori (+ 2 (* 3 top-minor)) debug stack$c)))
+
+(define stack$c-bindings ((stack$c stack$c-okp))
+  :enabled t
+  (stack$c-majori (* 2 (stack$c-top-frame stack$c)) stack$c))
+
+(define stack$c-minor-bindings ((stack$c stack$c-okp))
+  :enabled t
+  (b* ((top-minor (stack$c-top-minor-frame stack$c))
+       (index (* 3 top-minor)))
+    (stack$c-minori index stack$c)))
+
+(define stack$c-debug ((stack$c stack$c-okp))
+  :enabled t
+  (stack$c-majori (+ 1 (* 2 (stack$c-top-frame stack$c))) stack$c))
+
+(define stack$c-minor-debug ((stack$c stack$c-okp))
+  :enabled t
+  (b* ((top-minor (stack$c-top-minor-frame stack$c))
+       (index (+ 2 (* 3 top-minor))))
+    (stack$c-minori index stack$c)))
+
+(define stack$c-scratchlen ((stack$c stack$c-okp))
+  :enabled t
+  (b* ((top-minor (stack$c-top-minor-frame stack$c))
+       (index (+ 1 (* 3 top-minor))))
+    (len (stack$c-minori index stack$c))))
+
+
+(local (defthm true-listp-when-gl-objectlist-p-rw
+         (implies (gl-objectlist-p x)
+                  (true-listp x))))
+
+(define stack$c-pop-scratch ((n natp)
+                             (stack$c stack$c-okp))
+  :enabled t
+  :guard (<= n (stack$c-scratchlen stack$c))
+  (b* ((top-minor (stack$c-top-minor-frame stack$c))
+       (index (+ 1 (* 3 top-minor))))
+    (update-stack$c-minori index (nthcdr n (stack$c-minori index stack$c)) stack$c)))
+
+(define stack$c-scratch ((stack$c stack$c-okp))
+  :enabled t
+  (b* ((top-minor (stack$c-top-minor-frame stack$c))
+       (index (+ 1 (* 3 top-minor))))
+    (stack$c-minori index stack$c)))
+
+(local (defthm bound-when-stack$c-top-minorp
+         (implies (and (stack$c-top-minorp x)
+                       (< (nfix n) (len x)))
+                  (< (nth-nat n x) (expt 2 32)))
+         :hints(("Goal" :in-theory (enable nth-nat nth len)))
+         :rule-classes :linear))
+
+(define stack$c-pop-minor-frame ((stack$c stack$c-okp))
+  :enabled t
+  :guard (< 1 (stack$c-minor-frames stack$c))
+  (b* ((top-major (stack$c-top-frame stack$c))
+       (top-minor (stack$c-top-minor-frame stack$c))
+       (offset (* 3 top-minor))
+       (stack$c (update-stack$c-minori offset nil stack$c))
+       (stack$c (update-stack$c-minori (+ 1 offset) nil stack$c))
+       (stack$c (update-stack$c-minori (+ 2 offset) nil stack$c))
+       (new-top-minor (+ -1 top-minor))
+       (stack$c (update-stack$c-top-minori top-major new-top-minor stack$c)))
+    (update-stack$c-top-minor-frame new-top-minor stack$c)))
+
+(define stack$c-pop-frame ((stack$c stack$c-okp))
+  :enabled t
+  :guard (and (< 1 (stack$c-frames stack$c))
+              (eql 1 (stack$c-minor-frames stack$c)))
+  :prepwork ((local (defthm nth-nat-upper-bound-by-nth-dumb
+                      (implies (and (< (nth n x) b)
+                                    (posp b))
+                               (< (+ -1 (nth-nat n x)) b))
+                      :hints(("Goal" :in-theory (enable nth-nat nfix))))))
+  (b* ((top-major (stack$c-top-frame stack$c))
+       (top-minor (stack$c-top-minor-frame stack$c))
+       (minor-offset (* 3 top-minor))
+       (stack$c (update-stack$c-minori minor-offset nil stack$c))
+       (stack$c (update-stack$c-minori (+ 1 minor-offset) nil stack$c))
+       (stack$c (update-stack$c-minori (+ 2 minor-offset) nil stack$c))
+       (major-offset (* 2 top-major))
+       (stack$c (update-stack$c-majori major-offset nil stack$c))
+       (stack$c (update-stack$c-majori (+ 1 major-offset) nil stack$c))
+       (stack$c (update-stack$c-top-frame (+ -1 top-major) stack$c)))
+    (update-stack$c-top-minor-frame (+ -1 top-minor) stack$c)))
+
+
+(define stack$c-build-minor-frames ((bottom natp) (top natp) (stack$c stack$c-okp))
+  :returns (frames minor-stack-p)
+  :measure (lnfix top)
+  :ruler-extenders (cons)
+  :guard (<= (+ 3 (* 3 top)) (stack$c-minor-length stack$c))
+  :enabled t
+  (cons (make-minor-frame :bindings (stack$c-minori (* 3 (lnfix top)) stack$c)
+                          :scratch (stack$c-minori (+ 1 (* 3 (lnfix top))) stack$c)
+                          :debug (stack$c-minori (+ 2 (* 3 (lnfix top))) stack$c))
+        (and (< (lnfix bottom) (lnfix top))
+             (stack$c-build-minor-frames bottom (1- (lnfix top)) stack$c)))
+  ///
+  (defthm len-of-stack$c-build-minor-frames
+    (equal (len (stack$c-build-minor-frames bottom top stack$c))
+           (pos-fix (+ 1 (- (nfix top) (nfix bottom)))))
+    :hints(("Goal" :in-theory (enable len pos-fix)))))
+
+(define stack$c-build-major-frames ((top natp) (stack$c stack$c-okp))
+  :returns (frames major-stack-p)
+  :measure (lnfix top)
+  :ruler-extenders (cons)
+  :guard (<= top (stack$c-top-frame stack$c))
+  :guard-hints (("goal" :use ((:instance stack$c-top-minor-ordered-necc
+                               (i top) (j (stack$c-top-frame stack$c))))
+                 :in-theory (disable stack$c-top-minor-ordered-necc)))
+  :enabled t
+  (cons (make-major-frame :bindings (stack$c-majori (* 2 (lnfix top)) stack$c)
+                          :debug (stack$c-majori (+ 1 (* 2 (lnfix top))) stack$c)
+                          :minor-stack (stack$c-build-minor-frames
+                                        (if (zp top)
+                                            0
+                                          (+ 1 (stack$c-top-minori (1- (lnfix top)) stack$c)))
+                                        (stack$c-top-minori (lnfix top) stack$c)
+                                        stack$c))
+        (and (posp top)
+             (stack$c-build-major-frames (1- (lnfix top)) stack$c)))
+  ///
+  
+  (defthm len-of-stack$c-build-major-frames
+    (equal (len (stack$c-build-major-frames top stack$c))
+           (+ 1 (nfix top)))
+    :hints(("Goal" :in-theory (enable len)))))
+
+(local (defsection range-nat-equiv
+         (defthmd nth-nat-when-range-nat-equiv
+           (implies (and (stobjs::range-nat-equiv start num x y)
+                         (<= (nfix start) (nfix n))
+                         (< (nfix n) (+ (nfix start) (nfix num))))
+                    (equal (nth-nat n x) (nth-nat n y)))
+           :hints(("Goal" :in-theory (enable nth-nat stobjs::nth-when-range-nat-equiv))))
+
+         (defthm range-nat-equiv-by-badguy-nth-nat
+           (let ((badguy (stobjs::range-nat-equiv-badguy start num x y)))
+             (implies (equal (nth-nat badguy x) (nth-nat badguy y))
+                      (stobjs::range-nat-equiv start num x y)))
+           :hints (("Goal" :in-theory (enable nth-nat))))
+           
+
+         (defthm range-nat-equiv-by-badguy-literal-nth-nat
+           (let ((badguy (stobjs::range-nat-equiv-badguy start num x y)))
+             (implies (acl2::rewriting-positive-literal `(stobjs::range-nat-equiv ,start ,num ,x ,y))
+                      (iff (stobjs::range-nat-equiv start num x y)
+                           (or (not (< badguy (+ (nfix start) (nfix num))))
+                               (equal (nth-nat badguy x) (nth-nat badguy y))))))
+           :hints(("Goal" :in-theory (enable stobjs::range-nat-equiv-by-badguy-literal
+                                             stobjs::nth-when-range-nat-equiv
+                                             nth-nat))))
+
+         (defthm range-nat-equiv-by-superrange1
+           (implies (and (stobjs::range-nat-equiv min1 max1 x y)
+                         (<= (nfix min1) (nfix min))
+                         (<= (+ (nfix min) (nfix max))
+                             (+ (nfix min1) (nfix max1))))
+                    (stobjs::range-nat-equiv min max x y))
+           :hints(("Goal" :in-theory (disable range-nat-equiv-by-badguy-literal-nth-nat))))
+
+         (defthm range-nat-equiv-when-range-nat-equiv1
+           (implies (stobjs::range-nat-equiv start num x y)
+                    (stobjs::range-nat-equiv start num x y)))))
+
+(local
+ (defthm stack$c-build-minor-frames-of-update
+   (implies (and (bind-free (stobjs::bind-updater-independence-prev-stobj new mfc state))
+                 (syntaxp (not (equal new old)))
+                 (<= (nfix bottom) (nfix top))
+                 (stobjs::range-equal (* 3 (nfix bottom))
+                                      (+ 3 (* 3 (- (nfix top) (nfix bottom))))
+                                      (nth *stack$c-minori* new)
+                                      (nth *stack$c-minori* old)))
+            (equal (stack$c-build-minor-frames bottom top new)
+                   (stack$c-build-minor-frames bottom top old)))
+   :hints (("goal" :induct (stack$c-build-minor-frames bottom top new)
+            :expand ((:free (new) (stack$c-build-minor-frames bottom top new)))
+            :in-theory (enable stobjs::nth-when-range-equal)))))
+
+
+(local
+ (defsection stack$c-build-major-frames-of-update
+   (local (defthm zp-forwrad-to-nat-equiv-0
+            (implies (zp x)
+                     (acl2::nat-equiv x 0))
+            :rule-classes :forward-chaining))
+
+   (local
+    (defthmd stack$c-build-major-frames-of-update-lemma
+      (let ((top-minor (nth-nat top (nth *stack$c-top-minori1* old))))
+        (implies (and (bind-free (stobjs::bind-updater-independence-prev-stobj new mfc state))
+                      (stack$c-top-minor-ordered old)
+                      (<= (nfix top) (stack$c-top-frame old))
+                      (stobjs::range-equal 0 (+ 2 (* 2 (nfix top)))
+                                           (nth *stack$c-majori* new)
+                                           (nth *stack$c-majori* old))
+                      (stobjs::range-nat-equiv 0 (+ 1 (nfix top))
+                                               (nth *stack$c-top-minori1* new)
+                                               (nth *stack$c-top-minori1* old))
+                      ;; (equal top-minor (nth-nat top (nth *stack$c-top-minori1* old)))
+                      (stobjs::range-equal 0 (+ 3 (* 3 top-minor))
+                                           (nth *stack$c-minori* new)
+                                           (nth *stack$c-minori* old)))
+                 (equal (stack$c-build-major-frames top new)
+                        (stack$c-build-major-frames top old))))
+      :hints (("goal" :induct (stack$c-build-major-frames top new)
+               :expand ((:free (new) (stack$c-build-major-frames top new)))
+               :in-theory (enable stobjs::nth-when-range-equal
+                                  nth-nat-when-range-nat-equiv)
+               :do-not-induct t))))
+
+   (defthm stack$c-build-major-frames-of-update
+     (implies (and (bind-free (stobjs::bind-updater-independence-prev-stobj new mfc state))
+                   (syntaxp (not (equal new old)))
+                   (stack$c-top-minor-ordered old)
+                   (<= (nfix top) (stack$c-top-frame old))
+                   (stobjs::range-equal 0 (+ 2 (* 2 (nfix top)))
+                                        (nth *stack$c-majori* new)
+                                        (nth *stack$c-majori* old))
+                   (stobjs::range-nat-equiv 0 (+ 1 (nfix top))
+                                            (nth *stack$c-top-minori1* new)
+                                            (nth *stack$c-top-minori1* old))
+                   (equal top-minor (nth-nat top (nth *stack$c-top-minori1* old)))
+                   (stobjs::range-equal 0 (+ 3 (* 3 top-minor))
+                                        (nth *stack$c-minori* new)
+                                        (nth *stack$c-minori* old)))
+              (equal (stack$c-build-major-frames top new)
+                     (stack$c-build-major-frames top old)))
+     :hints (("goal" :use stack$c-build-major-frames-of-update-lemma)))))
+
+
+(define stack$c-extract ((stack$c stack$c-okp))
+  :enabled t
+  (stack$c-build-major-frames (stack$c-top-frame stack$c) stack$c))
+     
+
+
+
+
+;; (local (include-book "std/util/termhints" :dir :system))
+;; (local (include-book "std/basic/arith-equivs" :dir :system))
+;; (local (in-theory (enable* acl2::arith-equiv-forwarding)))
+
+
+;; (local (include-book "std/stobjs/updater-independence" :dir :system))
+
+;; (local (defsection range-nat-equiv
+;;          (defthmd nth-nat-when-range-nat-equiv
+;;            (implies (and (stobjs::range-nat-equiv start num x y)
+;;                          (<= (nfix start) (nfix n))
+;;                          (< (nfix n) (+ (nfix start) (nfix num))))
+;;                     (equal (nth-nat n x) (nth-nat n y)))
+;;            :hints(("Goal" :in-theory (enable nth-nat stobjs::nth-when-range-nat-equiv))))
+
+;;          (defthm range-nat-equiv-by-badguy-nth-nat
+;;            (let ((badguy (stobjs::range-nat-equiv-badguy start num x y)))
+;;              (implies (equal (nth-nat badguy x) (nth-nat badguy y))
+;;                       (stobjs::range-nat-equiv start num x y)))
+;;            :hints (("Goal" :in-theory (enable nth-nat))))
+           
+
+;;          (defthm range-nat-equiv-by-badguy-literal-nth-nat
+;;            (let ((badguy (stobjs::range-nat-equiv-badguy start num x y)))
+;;              (implies (acl2::rewriting-positive-literal `(stobjs::range-nat-equiv ,start ,num ,x ,y))
+;;                       (iff (stobjs::range-nat-equiv start num x y)
+;;                            (or (not (< badguy (+ (nfix start) (nfix num))))
+;;                                (equal (nth-nat badguy x) (nth-nat badguy y))))))
+;;            :hints(("Goal" :in-theory (enable stobjs::range-nat-equiv-by-badguy-literal
+;;                                              stobjs::nth-when-range-nat-equiv
+;;                                              nth-nat))))
+
+;;          (defthm range-nat-equiv-by-superrange1
+;;            (implies (and (stobjs::range-nat-equiv min1 max1 x y)
+;;                          (<= (nfix min1) (nfix min))
+;;                          (<= (+ (nfix min) (nfix max))
+;;                              (+ (nfix min1) (nfix max1))))
+;;                     (stobjs::range-nat-equiv min max x y))
+;;            :hints(("Goal" :in-theory (disable range-nat-equiv-by-badguy-literal-nth-nat))))
+
+;;          (defthm range-nat-equiv-when-range-nat-equiv1
+;;            (implies (stobjs::range-nat-equiv start num x y)
+;;                     (stobjs::range-nat-equiv start num x y)))))
+
+;; (local
+;;  (define major-frame-for-minor-frame-indexp ((j natp) (n natp) stack$c)
+;;    :verify-guards nil
+;;    :non-executable t
+;;    (b* ((n (nfix n))
+;;         (j (nfix j)))
+;;      (and (or (equal j 0)
+;;               (< (nth-nat (+ -1 j) (nth *stack$c-top-minori1* stack$c)) n))
+;;           (<= n (nth-nat j (nth *stack$c-top-minori1* stack$c)))))
+;;    ///
+;;    (fty::deffixequiv major-frame-for-minor-frame-indexp)
+
+;;    (defthmd major-frame-for-minor-frame-index-uniquep
+;;      (implies (and (major-frame-for-minor-frame-indexp j n stack$c)
+;;                    (stack$c-top-minor-ordered stack$c)
+;;                    (<= (nfix j) (nth-nat *stack$c-top-frame1* stack$c))
+;;                    (<= (nfix j1) (nth-nat *stack$c-top-frame1* stack$c)))
+;;               (equal (major-frame-for-minor-frame-indexp j1 n stack$c)
+;;                      (equal (nfix j1) (nfix j))))
+;;      :hints (("goal" ;; :cases ((major-frame-for-minor-frame-indexp j1 n stack$c))
+;;               :in-theory (disable stack$c-top-minor-ordered-necc))
+;;              (acl2::use-termhint
+;;               (if (major-frame-for-minor-frame-indexp j1 n stack$c)
+;;                   (if (< (nfix j1) (nfix j))
+;;                       '(:use ((:instance acl2::mark-clause-is-true (x j1-less))
+;;                               (:instance stack$c-top-minor-ordered-necc
+;;                                (i (nfix j1)) (j (+ -1 (nfix j))))))
+;;                     '(:use ((:instance acl2::mark-clause-is-true (x j1-greater))
+;;                             (:instance stack$c-top-minor-ordered-necc
+;;                              (i (nfix j)) (j (+ -1 (nfix j1)))))))
+;;                 '(:in-theory (disable major-frame-for-minor-frame-indexp))))))))
+
+
+;; ;; (local (include-book "arithmetic/top" :Dir :system))
+
+;; (local
+;;  (define find-major-frame-for-minor-frame-index-aux ((n natp) (j natp) stack$c)
+;;    :verify-guards nil
+;;    :non-executable t
+;;    :measure (nfix (- (nth-nat *stack$c-top-frame1* stack$c) (nfix j)))
+;;    :returns (maj-frame natp :rule-classes :type-prescription)
+;;    (if (zp (- (nth-nat *stack$c-top-frame1* stack$c) (nfix j)))
+;;        (nth-nat *stack$c-top-frame1* stack$c)
+;;      (let ((n (nfix n)))
+;;        (if (<= n (nth-nat j (nth *stack$c-top-minori1* stack$c)))
+;;            (nfix j)
+;;          (find-major-frame-for-minor-frame-index-aux n (+ 1 (nfix j)) stack$c))))
+;;    ///
+
+;;    (fty::deffixequiv find-major-frame-for-minor-frame-index-aux)
+;;    (local (defthm find-major-frame-gte-j
+;;             (implies (<= (nfix j) (nth-nat *stack$c-top-frame1* stack$c))
+;;                      (<= (nfix j) (find-major-frame-for-minor-frame-index-aux n j stack$c)))
+;;             :rule-classes :linear))
+
+;;    (local (defthm find-major-frame-lte-top-frame
+;;             (<= (find-major-frame-for-minor-frame-index-aux n j stack$c)
+;;                 (nth-nat *stack$c-top-frame1* stack$c))
+;;             :rule-classes :linear))
+
+;;    ;; (local (defthm minor-frame-of-find-major-frame-linear
+;;    ;;          (implies (<= (nfix j) (nth-nat *stack$c-top-frame1* stack$c))
+;;    ;;                   (<= (nth-nat j (nth *stack$c-top-minori1* stack$c))
+;;    ;;                       (nth-nat (find-major-frame-for-minor-frame-index-aux n j stack$c)
+;;    ;;                                (nth *stack$c-top-minori1* stack$c))
+
+;;    (defthm major-frame-for-minor-frame-indexp-of-find-major-frame-aux
+;;      (b* ((maj (find-major-frame-for-minor-frame-index-aux n j stack$c))
+;;           (top-minor (nth-nat (nth-nat *stack$c-top-frame1* stack$c) (nth *stack$c-top-minori1* stack$c))))
+;;        (implies (and (stack$c-top-minor-ordered stack$c)
+;;                      (<= (nfix j) (nth-nat *stack$c-top-frame1* stack$c))
+;;                      (or (zp j)
+;;                          (< (nth-nat (+ -1 j) (nth *stack$c-top-minori1* stack$c)) (nfix n)))
+;;                      (<= (nfix n) top-minor))
+;;                 (major-frame-for-minor-frame-indexp
+;;                  maj n stack$c)))
+;;      :hints(("Goal" :in-theory (enable major-frame-for-minor-frame-indexp)
+;;              :induct (find-major-frame-for-minor-frame-index-aux n j stack$c))
+;;             ;; (and stable-under-simplificationp
+;;             ;;      '(:use ((:instance stack$c-top-minor-ordered-necc
+;;             ;;               (j (+ -1 (nfix j))) (i (+ -1 (nth-nat *stack$c-top-frame1* stack$c)))))
+;;             ;;        :in-theory (disable stack$c-top-minor-ordered-necc)))
+;;             ))
+
+;;    (defthm find-major-frame-for-minor-frame-index-aux-of-update
+;;      (implies (bind-free (acl2::prev-stobj-binding new 'old mfc state))
+;;               (let ((maj (find-major-frame-for-minor-frame-index-aux n j old)))
+;;                 (implies (and (stobjs::range-nat-equiv j (+ 1 maj (- j)) (nth *stack$c-top-minori1* new) (nth *stack$c-top-minori1* old))
+;;                               (<= maj (nth-nat *stack$c-top-frame1* new)))
+;;                          (equal (find-major-frame-for-minor-frame-index-aux n j new)
+;;                                 maj))))
+;;      :hints (("goal" :induct (find-major-frame-for-minor-frame-index-aux n j old)
+;;               :expand ((:free (x) (find-major-frame-for-minor-frame-index-aux n j x)))
+;;               :in-theory (enable nth-nat-when-range-nat-equiv))))))
+
+
+;; (local (define find-major-frame-for-minor-frame-index ((n natp) stack$c)
+;;          :verify-guards nil
+;;          :non-executable t
+;;          :returns (maj-frame natp :rule-classes :type-prescription)
+;;          (find-major-frame-for-minor-frame-index-aux n 0 stack$c)
+;;          ///
+;;          (defthm major-frame-for-minor-frame-indexp-of-find-major-frame
+;;            (b* ((maj (find-major-frame-for-minor-frame-index n stack$c))
+;;                 (top-minor (nth-nat (nth-nat *stack$c-top-frame1* stack$c) (nth *stack$c-top-minori1* stack$c))))
+;;              (implies (and (stack$c-top-minor-ordered stack$c)
+;;                            (<= (nfix n) top-minor))
+;;                       (major-frame-for-minor-frame-indexp
+;;                        maj n stack$c))))
+
+;;          (local (in-theory (disable find-major-frame-for-minor-frame-index
+;;                                     major-frame-for-minor-frame-indexp-of-find-major-frame)))
+
+;;          (defthm upper-bound-by-find-major-frame-for-minor-frame-index
+;;            (b* ((maj (find-major-frame-for-minor-frame-index n stack$c))
+;;                 (top-minor (nth-nat (nth-nat *stack$c-top-frame1* stack$c) (nth *stack$c-top-minori1* stack$c))))
+;;              (implies (and (stack$c-top-minor-ordered stack$c)
+;;                            (<= (nfix n) top-minor))
+;;                       (<= (nfix n) (nth-nat maj (nth *stack$c-top-minori1* stack$c)))))
+;;            :hints (("goal" :use major-frame-for-minor-frame-indexp-of-find-major-frame
+;;                     :in-theory (enable major-frame-for-minor-frame-indexp)))
+;;            :rule-classes :linear)
+
+;;          (defthm lower-bound-by-find-major-frame-for-minor-frame-index
+;;            (b* ((maj (find-major-frame-for-minor-frame-index n stack$c))
+;;                 (top-minor (nth-nat (nth-nat *stack$c-top-frame1* stack$c) (nth *stack$c-top-minori1* stack$c))))
+;;              (implies (and (stack$c-top-minor-ordered stack$c)
+;;                            (<= (nfix n) top-minor)
+;;                            (not (equal maj 0)))
+;;                       (< (nth-nat (+ -1 maj) (nth *stack$c-top-minori1* stack$c)) (nfix n))))
+;;            :hints (("goal" :use major-frame-for-minor-frame-indexp-of-find-major-frame
+;;                     :in-theory (enable major-frame-for-minor-frame-indexp)))
+;;            :rule-classes :linear)
+
+;;          (defthm find-major-frame-for-minor-frame-index-of-update
+;;            (implies (bind-free (prev-stobj-binding new 'old mfc state))
+;;                     (let ((maj (find-major-frame-for-minor-frame-index n old)))
+;;                       (implies (and (stobjs::range-nat-equiv 0 (+ 1 maj) (nth *stack$c-top-minori1* new) (nth *stack$c-top-minori1* old))
+;;                                     (<= maj (nth-nat *stack$c-top-frame1* new)))
+;;                                (equal (find-major-frame-for-minor-frame-index n new)
+;;                                       maj))))))
+
+
+
+
+
+
+(local
+ (progn
+   (define stack-corr (stack$c stack$a)
+     :non-executable t
+     :enabled t
+     :verify-guards nil
+     (and (stack$c-okp stack$c)
+          (equal (stack$c-build-major-frames (stack$c-top-frame stack$c) stack$c) stack$a)))
+
+
+   (defthm nth-of-cons-split
+     (equal (nth n (cons a b))
+            (if (zp n)
+                a
+              (nth (+ -1 n) b)))
+     :hints(("Goal" :in-theory (enable nth))))
+
+   (defthm max-when-gte
+     (implies (and (<= a b)
+                   (integerp a) (integerp b))
+              (equal (max a b) b))
+     :hints(("Goal" :in-theory (enable max))))
+
+
+   (defthm equal-plus-consts
+     (implies (syntaxp (and (quotep a) (quotep b)))
+              (equal (equal (+ a c) (+ b d))
+                     (equal (+ (+ (- b) a) c) (fix d)))))
+
+   (defthm equal-const-plus-3*
+     (implies (syntaxp (quotep c))
+              (equal (equal (+ c (* 3 x)) (* 3 y))
+                     (equal (+ (/ c 3) x) (fix y)))))
+
+
+   (defthm equal-const-plus-2*
+     (implies (syntaxp (quotep c))
+              (equal (equal (+ c (* 2 x)) (* 2 y))
+                     (equal (+ (/ c 2) x) (fix y)))))
+
+
+   (in-theory (disable (stack$c-build-major-frames)
+                       (stack$c-build-minor-frames)))
+
+
+   (defthm stack$c-build-minor-frames-of-update-hack
+     (implies (and (bind-free '((old . stack$c)))
+                   (syntaxp (not (equal new old)))
+                   (<= (nfix bottom) (nfix top))
+                   (stobjs::range-equal (* 3 (nfix bottom))
+                                        (+ 3 (* 3 (- (nfix top) (nfix bottom))))
+                                        (nth *stack$c-minori* new)
+                                        (nth *stack$c-minori* old)))
+              (equal (stack$c-build-minor-frames bottom top new)
+                     (stack$c-build-minor-frames bottom top old)))
+     :hints (("goal" :use stack$c-build-minor-frames-of-update
+              :in-theory (disable stack$c-build-minor-frames-of-update))))
+
+   (defthm stack$c-build-major-frames-of-update-hack
+     (implies (and (bind-free '((old . stack$c)))
+                   (syntaxp (not (equal new old)))
+                   (stack$c-top-minor-ordered old)
+                   (<= (nfix top) (stack$c-top-frame old))
+                   (stobjs::range-equal 0 (+ 2 (* 2 (nfix top)))
+                                        (nth *stack$c-majori* new)
+                                        (nth *stack$c-majori* old))
+                   (stobjs::range-nat-equiv 0 (+ 1 (nfix top))
+                                            (nth *stack$c-top-minori1* new)
+                                            (nth *stack$c-top-minori1* old))
+                   (equal top-minor (nth-nat top (nth *stack$c-top-minori1* old)))
+                   (stobjs::range-equal 0 (+ 3 (* 3 top-minor))
+                                        (nth *stack$c-minori* new)
+                                        (nth *stack$c-minori* old)))
+              (equal (stack$c-build-major-frames top new)
+                     (stack$c-build-major-frames top old)))
+     :hints (("goal" :use stack$c-build-major-frames-of-update
+              :in-theory (disable stack$c-build-major-frames-of-update))))
+
+   (defthm nth-0-stack$c-build-major-frames
+     (equal (nth 0 (stack$c-build-major-frames top stack$c))
+            (car (stack$c-build-major-frames top stack$c))))
+
+   (defthm car-stack$c-build-major-frames
+     (equal (car (stack$c-build-major-frames top stack$c))
+            (MAKE-MAJOR-FRAME
+             :BINDINGS (STACK$C-MAJORI (* 2 (LNFIX TOP))
+                                       STACK$C)
+             :DEBUG (STACK$C-MAJORI (+ 1 (* 2 (LNFIX TOP)))
+                                    STACK$C)
+             :MINOR-STACK
+             (STACK$C-BUILD-MINOR-FRAMES
+              (IF (ZP TOP)
+                  0
+                  (+ 1
+                     (STACK$C-TOP-MINORI (1- (LNFIX TOP))
+                                         STACK$C)))
+              (STACK$C-TOP-MINORI (LNFIX TOP) STACK$C)
+              STACK$C))))
+
+   (defthm stack$c-build-major-frames-0
+     (equal (stack$c-build-major-frames 0 stack$c)
+            (list (MAKE-MAJOR-FRAME
+                   :BINDINGS (STACK$C-MAJORI 0
+                                             STACK$C)
+                   :DEBUG (STACK$C-MAJORI 1
+                                          STACK$C)
+                   :MINOR-STACK
+                   (STACK$C-BUILD-MINOR-FRAMES 0
+                                               (STACK$C-TOP-MINORI 0 STACK$C)
+                                               STACK$C)))))
+
+   (defthm stack$c-build-major-frames-plus1
+     (implies (natp top)
+              (equal (stack$c-build-major-frames (+ 1 top) stack$c)
+                     (cons (let ((top (+ 1 top)))
+                             (MAKE-MAJOR-FRAME
+                              :BINDINGS (STACK$C-MAJORI (* 2 (LNFIX TOP))
+                                                        STACK$C)
+                              :DEBUG (STACK$C-MAJORI (+ 1 (* 2 (LNFIX TOP)))
+                                                     STACK$C)
+                              :MINOR-STACK
+                              (STACK$C-BUILD-MINOR-FRAMES
+                               (IF (ZP TOP)
+                                   0
+                                   (+ 1
+                                      (STACK$C-TOP-MINORI (1- (LNFIX TOP))
+                                                          STACK$C)))
+                               (STACK$C-TOP-MINORI (LNFIX TOP) STACK$C)
+                               STACK$C)))
+                           (stack$c-build-major-frames top stack$c)))))
+
+   (defthm nth-0-stack$C-build-minor-frames
+     (equal (nth 0 (stack$c-build-minor-frames bottom top stack$c))
+            (car (stack$c-build-minor-frames bottom top stack$c))))
+
+   (defthm car-stack$C-build-minor-frames
+     (equal (car (stack$c-build-minor-frames bottom top stack$c))
+            (MAKE-MINOR-FRAME
+             :BINDINGS (STACK$C-MINORI (* 3 (LNFIX TOP))
+                                       STACK$C)
+             :SCRATCH (STACK$C-MINORI (+ 1 (* 3 (LNFIX TOP)))
+                                      STACK$C)
+             :DEBUG (STACK$C-MINORI (+ 2 (* 3 (LNFIX TOP)))
+                                    STACK$C))))
+
+   (defthm stack$C-build-minor-frames-zero
+     (equal (stack$c-build-minor-frames top top stack$c)
+            (list (MAKE-MINOR-FRAME
+                   :BINDINGS (STACK$C-MINORI (* 3 (LNFIX TOP))
+                                             STACK$C)
+                   :SCRATCH (STACK$C-MINORI (+ 1 (* 3 (LNFIX TOP)))
+                                            STACK$C)
+                   :DEBUG (STACK$C-MINORI (+ 2 (* 3 (LNFIX TOP)))
+                                          STACK$C)))))
+
+   (defthm stack$C-build-minor-frames-plus-1
+     (implies (and (<= (nfix bottom) top)
+                   (natp top))
+              (equal (stack$c-build-minor-frames bottom (+ 1 top) stack$c)
+                     (cons (let ((top (+ 1 top)))
+                             (MAKE-MINOR-FRAME
+                              :BINDINGS (STACK$C-MINORI (* 3 (LNFIX TOP))
+                                                        STACK$C)
+                              :SCRATCH (STACK$C-MINORI (+ 1 (* 3 (LNFIX TOP)))
+                                                       STACK$C)
+                              :DEBUG (STACK$C-MINORI (+ 2 (* 3 (LNFIX TOP)))
+                                                     STACK$C)))
+                           (stack$c-build-minor-frames bottom top stack$c)))))
+
+   (defthm stack$c-top-minor-ordered-lemma
+     (implies (and (stack$c-top-minor-ordered stack$c)
+                   (natp i)
+                   (integerp j)
+                   (< i j)
+                   (<= j (stack$c-top-frame stack$c))
+                   (< 1 (- (nth-nat j (nth *stack$c-top-minori1* stack$C))
+                           (nth-nat (+ -1 j) (nth *stack$c-top-minori1* stack$C)))))
+              (< (nth-nat i (nth *stack$c-top-minori1* stack$C))
+                 (+ -1 (nth-nat j (nth *stack$c-top-minori1* stack$c)))))
+     :hints (("goal" :use ((:instance stack$c-top-minor-ordered-necc
+                            (i i) (j (+ -1 j))))
+              :in-theory (disable stack$c-top-minor-ordered-necc))))
+
+   
+
+   (include-book "clause-processors/generalize" :dir :system)
+   (include-book "clause-processors/find-subterms" :dir :system)
+
+   (set-default-hints
+    '((and stable-under-simplificationp
+           (let* ((lit (car (last clause)))
+                  (hint
+                   (cond ((member (car lit)
+                                  '(stack$c-major-frames-welltyped
+                                    stack$c-minor-frames-welltyped
+                                    stack$c-major-frames-bounded
+                                    stack$c-minor-frames-bounded
+                                    stack$c-top-minor-ordered
+                                    ))
+                          (let ((witness-sym (intern-in-package-of-symbol
+                                              (concatenate 'string (symbol-name (car lit)) "-WITNESS")
+                                              (car lit)))
+                                (witness-sym2 (intern-in-package-of-symbol
+                                               (concatenate 'string (symbol-name (car lit)) "-WITNESS2")
+                                               (car lit))))
+                            `(:computed-hint-replacement
+                              ((let* ((call (acl2::find-call-lst ',witness-sym clause)))
+                                 (and call
+                                      `(:clause-processor
+                                        (acl2::generalize-with-alist-cp
+                                         clause '((,call . ,',witness-sym)
+                                                  ((mv-nth '2 ,call) . ,',witness-sym2)
+                                                  ))))))
+                              :expand (,lit))))
+                         (t ;; (acl2::find-call 'stack$c-build-major-frames lit)
+                          `(;; :computed-hint-replacement t
+                            :expand ((:free (stack$c1)
+                                      (stack$c-build-major-frames (nth-nat *stack$c-top-frame1* stack$c)
+                                                                  stack$c1))
+                                     (:free (bottom stack$c1)
+                                      (stack$c-build-minor-frames bottom
+                                                                  (nth-nat (nth-nat *stack$c-top-frame1* stack$c)
+                                                                           (nth *stack$c-top-minori1* stack$c))
+                                                                  stack$c1))
+                                     (:free (stack$c1)
+                                      (stack$c-build-minor-frames 0
+                                                                  (nth-nat 0
+                                                                           (nth *stack$c-top-minori1* stack$c))
+                                                                  stack$c1))))))))
+             ;; (prog2$ (cw "hint: ~x0~%" hint)
+             hint))))
+
+   (in-theory (disable stack$c-build-minor-frames
+                       stack$c-build-major-frames
+                       cons-equal
+                       true-listp-update-nth
+                       acl2::nth-when-too-large-cheap
+                       ;; len-stack-when-atom-cdr
+                       stack$c-top-minorp
+                       unsigned-byte-p
+                       acl2::nfix-when-not-natp
+                       acl2::nth-when-atom))
+   
+   ))
+
+(defabsstobj-events stack
+  :concrete stack$c
+  :corr-fn stack-corr
+  :recognizer (stackp :logic major-stack-p
+                      :exec stack$cp)
+  :creator (create-stack :logic create-stack$a
+                         :exec create-stack$c)
+  :exports ((stack-frames :logic stack$a-frames :exec stack$c-frames)
+            (stack-push-frame :logic stack$a-push-frame :exec stack$c-push-frame :protect t)
+            (stack-minor-frames :logic stack$a-minor-frames :exec stack$c-minor-frames)
+            (stack-push-minor-frame :logic stack$a-push-minor-frame :exec stack$c-push-minor-frame :protect t)
+            (stack-set-bindings :logic stack$a-set-bindings :exec stack$c-set-bindings)
+            (stack-add-binding :logic stack$a-add-binding :exec stack$c-add-binding)
+            (stack-set-debug :logic stack$a-set-debug :exec stack$c-set-debug)
+            (stack-set-minor-bindings :logic stack$a-set-minor-bindings :exec stack$c-set-minor-bindings)
+            (stack-add-minor-bindings :logic stack$a-add-minor-bindings :exec stack$c-add-minor-bindings)
+            (stack-push-scratch :logic stack$a-push-scratch :exec stack$c-push-scratch)
+            (stack-set-minor-debug :logic stack$a-set-minor-debug :exec stack$c-set-minor-debug)
+            (stack-bindings :logic stack$a-bindings :exec stack$c-bindings)
+            (stack-minor-bindings :logic stack$a-minor-bindings :exec stack$c-minor-bindings)
+            (stack-debug :logic stack$a-debug :exec stack$c-debug)
+            (stack-minor-debug :logic stack$a-minor-debug :exec stack$c-minor-debug)
+            (stack-scratchlen :logic stack$a-scratchlen :exec stack$c-scratchlen)
+            (stack-pop-scratch :logic stack$a-pop-scratch :exec stack$c-pop-scratch)
+            (stack-scratch :logic stack$a-scratch :exec stack$c-scratch)
+            (stack-pop-minor-frame :logic stack$a-pop-minor-frame :exec stack$c-pop-minor-frame :protect t)
+            (stack-pop-frame :logic stack$a-pop-frame :exec stack$c-pop-frame :protect t)
+            (stack-extract :logic stack$a-extract :exec stack$c-extract)))
